Isabroom.thy
@@ -12,7 +12,7 @@ datatype 'a command =
 | AssignVar var var
 | Load var var
 | Store var var
-| Malloc var
+| Malloc var var
 | Free var
 | BinOp binop var var
 | UnOp unop var
@@ -31,14 +31,55 @@ axiomatization entry :: CFG_node and exit :: CFG_node
 type_synonym 'a edge = "CFG_node \<times> 'a command \<times> CFG_node"
 type_synonym 'a cfg = "'a func \<times> 'a edge set"
 
+abbreviation can_allocate_from :: "blocks \<Rightarrow> loc \<Rightarrow> blockname \<Rightarrow> val \<Rightarrow> bool" where
+  "can_allocate_from B l n z \<equiv>
+    0<l \<and> \<comment> \<open>The location is not at null.\<close>
+    l < l + (loc64_ops.from_val z) \<and> \<comment> \<open>The allocated block does not wrap around.\<close>
+    \<comment> \<open>It doesn't overlap with any other block.\<close>
+    (\<forall>b\<in>set (raw_blocks B). \<not>(overlaps_with (n,l,l + (loc64_ops.from_val z)) b)) \<and>
+    (\<forall>b\<in>set (raw_blocks B). (case b of (n',_,_) \<Rightarrow> n'\<noteq>n)) \<comment> \<open>The name is new and unique\<close>"
+
 inductive semantics :: "pre_config \<Rightarrow> 'a command \<Rightarrow> pre_config option \<Rightarrow> bool" where
-  "fits k x \<Longrightarrow> semantics (S,B,M) (AssignConst x k) (Some (Stack ((lookup s)(x:=k)),B,M))"
-| "size x = size y \<Longrightarrow> semantics (S,B,M) (AssignVar x y) (Some (Stack ((lookup s)(x:=lookup s y)),B,M))"
-| "base B (loc64_ops.from_val (lookup s y)) = 0 \<or> 
-  (loc64_ops.from_val (lookup s y)) + (sizev x) > ende B (loc64_ops.from_val (lookup s y)) \<Longrightarrow>
-   semantics (S,B,M) (Load x y) None"
-| "\<not>(base B (loc64_ops.from_val (lookup s y)) = 0 \<or> 
-  (loc64_ops.from_val (lookup s y)) + (sizev x) > ende B (loc64_ops.from_val (lookup s y))) \<Longrightarrow>
-  
-  semantics (Stack ((lookup s)(x:=
+  "fits k x \<Longrightarrow> semantics (S,B,M) (AssignConst x k) (Some (Stack ((lookup S)(x:=k)),B,M))"
+| "size x = size y \<Longrightarrow> semantics (S,B,M) (AssignVar x y) (Some (Stack ((lookup S)(x:=lookup S y)),B,M))"
+| LoadFail: 
+  "\<comment> \<open>y does not point into any block, i.e. is an invalid location\<close>
+  base B (loc64_ops.from_val (lookup S y)) = 0 \<or>
+  \<comment> \<open>This load would read past the end of the block.\<close>
+  ((loc64_ops.from_val (lookup S y)) + (sizev x) > ende B (loc64_ops.from_val (lookup S y)) \<or> 
+  \<comment> \<open>This would read past the maximum location and wrap around.\<close>
+  (loc64_ops.from_val (lookup S y)) + (sizev x) \<le> (loc64_ops.from_val (lookup S y))) \<Longrightarrow>
+     semantics (S,B,M) (Load x y) None"
+| LoadSuccess: "\<lbrakk>\<not>(base B (loc64_ops.from_val (lookup S y)) = 0 \<or> 
+  ((loc64_ops.from_val (lookup S y)) + (sizev x) > ende B (loc64_ops.from_val (lookup S y)) \<or>
+  (loc64_ops.from_val (lookup S y)) + (sizev x) \<le> (loc64_ops.from_val (lookup S y))));
+  \<comment> \<open>The addressed memory cells are actually allocated.\<close>
+  access M (loc64_ops.from_val (lookup S y)) (size x) = Some v\<rbrakk> \<Longrightarrow> 
+    semantics (S,B,M) (Load x y) (Some (Stack ((lookup S)(x:=v)), B, M))"
+| StoreFail:
+  "\<comment> \<open>x does not point into any block, i.e. is an invalid location\<close>
+  base B (loc64_ops.from_val (lookup S x)) = 0 \<or>
+  \<comment> \<open>This store woudl write past the end of the block.\<close>
+  ((loc64_ops.from_val (lookup S x)) + (sizev y) > ende B (loc64_ops.from_val (lookup S x)) \<or> 
+  \<comment> \<open>This would write past the maximum location and wrap around.\<close>
+  (loc64_ops.from_val (lookup S x)) + (sizev y) \<le> (loc64_ops.from_val (lookup S x))) \<Longrightarrow>
+    semantics (S,B,M) (Store x y) None"
+| StoreSuccess: "\<not>(base B (loc64_ops.from_val (lookup S x)) = 0 \<or> 
+  ((loc64_ops.from_val (lookup S x)) + (sizev y) > ende B (loc64_ops.from_val (lookup S x)) \<or>
+  (loc64_ops.from_val (lookup S x)) + (sizev y) \<le> (loc64_ops.from_val (lookup S x)))) \<Longrightarrow> 
+    semantics (S,B,M) (Store x y) (Some (S, B, update_memory M (loc64_ops.from_val (lookup S x)) (lookup S y)))"
+| MallocError: "
+  \<comment> \<open>If we would allocate 0 bytes or x can't hold a pointer.\<close>
+  (\<forall>v\<in>set (lookup S z). v = 0) \<or> (size x \<noteq> loc_N_B) \<Longrightarrow> 
+  semantics (S,_,_) (Malloc x z) None"
+| MallocSuccessNull: "\<lbrakk>\<exists>v\<in>set (lookup S z). v \<noteq> 0; size x = loc_N_B\<rbrakk> \<Longrightarrow>
+  semantics (S,B,M) (Malloc x z) (Some (Stack ((lookup S)(x:=null x)),B,M))"
+| MallocSuccess: "\<lbrakk>\<exists>v\<in>set (lookup S z). v \<noteq> 0; size x = loc_N_B;
+  \<comment> \<open>l and n are new, k is arbitrary\<close>
+  can_allocate_from B l n (lookup S z); length k = length (lookup S z)\<rbrakk> \<Longrightarrow>
+  semantics (S,B,M) (Malloc x z) 
+    (Some (Stack ((lookup S)(x:=loc64_ops.to_val l)), 
+    Blocks ((n,l,l+(loc64_ops.from_val (lookup S z)))#raw_blocks B),
+    update_memory M l k))"
+
 end
